pulse/Pulse.Lib.C.Array.fsti
@@ -12,8 +12,28 @@ fn alloc_array u#a (#a:Type u#a) (sz:SizeT.t)
   ensures freeable_array r
   ensures A.pts_to_uninit r (SizeT.v sz)
 
-fn free_array u#a (#a:Type u#a) (r:array a)
+let free_array_pre (#a: Type u#a) (r: array a) : slprop =
+  A.pts_to_uninit_post r
+
+[@@pulse_intro]
+ghost fn intro_free_array_pre_init u#a (#a: Type u#a) (r: array a)
+  requires live r
+  ensures free_array_pre r
+{
+  A.to_mask r;
+  fold free_array_pre r;
+}
+
+[@@pulse_intro]
+ghost fn intro_free_array_pre_uninit u#a (#a: Type u#a) (r: array a)
   requires A.pts_to_uninit_post r
+  ensures free_array_pre r
+{
+  fold free_array_pre r;
+}
+
+fn free_array u#a (#a:Type u#a) (r:array a)
+  requires free_array_pre r
   requires freeable_array r
 
 fn calloc_array u#a (#a:Type u#a) {| has_zero_default a |} (sz:SizeT.t)
